added calc syntax, used it for poly1305_math

src/crypto/poly1305/x64/X64.Poly1305.Math_i.fst
@@ -5,7 +5,9 @@ open FStar.Tactics.Canon
 open FStar.Math.Lemmas
 open FStar.Math.Lib
 open FStar.Mul
+open Calc
 open X64.Vale.State_i   // needed for mem
+
 (*
 open FStar.Mul
 open FStar.UInt
@@ -18,7 +20,7 @@ lemma_BitwiseMul64()
 // private unfold let op_Star = op_Multiply
 
 // these settings make it super slow
-// #reset-options "--z3rlimit_factor 4 --z3rlimit 300 --z3cliopt smt.QI.EAGER_THRESHOLD=100 --z3cliopt smt.CASE_SPLIT=3 --z3cliopt smt.arith.nl=false --max_fuel 0 --max_ifuel 0 --smtencoding.elim_box true --eager_inference --smtencoding.nl_arith_repr wrapped --smtencoding.l_arith_repr native"
+// #reset-options "--z3cliopt smt.QI.EAGER_THRESHOLD=100 --z3cliopt smt.CASE_SPLIT=3 --z3cliopt smt.arith.nl=false --max_fuel 0 --max_ifuel 1 --smtencoding.elim_box true --smtencoding.nl_arith_repr wrapped --smtencoding.l_arith_repr native"
 
 
 let rec poly1305_heap_blocks (h:int) (pad:int) (r:int) (m:mem) (i:int) 
@@ -39,7 +41,7 @@ let rec poly1305_heap_blocks (h:int) (pad:int) (r:int) (m:mem) (i:int)
 *)
 
 
-#reset-options "--smtencoding.elim_box true --z3cliopt smt.arith.nl=true"
+#reset-options "--smtencoding.elim_box true --z3cliopt smt.arith.nl=true --max_fuel 1 --max_ifuel 1"
 
 val lemma_mul_div_comm: a:nat -> b:pos -> c:nat ->
     Lemma (requires (c % b = 0 /\ a % b = 0))
@@ -63,94 +65,59 @@ val lemma_mul_div_sep: a:nat -> b:pos -> c:nat ->
 	  (ensures (a*c)/b == a * (c/b))
 let lemma_mul_div_sep a b c = () 
 
-
-
-#reset-options "--smtencoding.elim_box true --z3cliopt smt.arith.nl=false"
-
 val swap_add: a:int -> b:int -> c:int -> Lemma
       (a + b + c = a + c + b)
 let swap_add a b c = ()
 
-// p used to be a refinement to p > 0 and r1 a nat.
-// There are some assumptions here, which will either go away when the library switches to ints everywhere (for division too)
-// or when we switch to nats (which is doable right away)
-let lemma_poly_multiply (n:int) (p:int) (r:int) (h:int) (r0:int) (r1:int) (h0:int) (h1:int) (h2:int) (s1:int) (d0:int) (d1:int) (d2:int) (hh:int) =
-    (* unfold h and r*)
-      assert ((h * r) == ((h2 * (n * n) + h1 * n + h0) * (r1*n + r0)));
-    
-    (* do some math using the canonizer *)
-      assert_by_tactic canon (((h2 * (n * n) + h1 * n + h0) * (r1*n + r0)) ==
-		       (h2 * n + h1) * ((n*n) * r1) + (h2 * r0) * (n * n) + (h1 * r0 + h0 * r1) * n + h0 * r0);
-    
-    (* proof that (n*n) = (p+5)/4*)
-      slash_star_axiom (n*n) 4 (p+5);
 
-    (* proof that ((p+5)/4)*r1 = (p+5)*(r1/4) *)
-      lemma_mul_div_comm (p+5) 4 r1;
+#reset-options "--z3cliopt smt.QI.EAGER_THRESHOLD=100 --z3cliopt smt.CASE_SPLIT=3 --z3cliopt smt.arith.nl=false --max_fuel 0 --max_ifuel 1 --smtencoding.elim_box true --smtencoding.nl_arith_repr wrapped --smtencoding.l_arith_repr native --z3rlimit 8"
 
-    (* use the proof above*)
-      assert ((h2 * n + h1) * ((n*n)*r1) = (h2 * n + h1) * ((p+5)*(r1/4)));
-      //TODO: check if this style of breaking the equalities is actually faster
-    (* we currently rely on Z3 to do the ``rewriting`` so we must be
-       very careful if we want to keep non-linear arithmetic off. *) 
-       
-      assert (((h2 * n + h1) * ((n*n)*r1)) + (h2 * r0) * (n * n) + (h1 * r0 + h0 * r1) * n + h0 * r0 == 
-      	   ((h2 * n + h1) * ((p+5)*(r1/4)) + (h2 * r0) * (n * n) + (h1 * r0 + h0 * r1) * n + h0 * r0));
-      assert (h*r == (h2 * n + h1) * ((p+5)*(r1/4)) + (h2 * r0) * (n * n) + (h1 * r0 + h0 * r1) * n + h0 * r0);
-
-    // helper_lemma_2 does all the work but takes 100s. It times out if no helper is used.
-    let helper_lemma_2 (x:int) : Lemma 
-       (ensures ((h2 * n + h1) * ((p+5) * x) + (h2 * r0) * (n * n) + (h1 * r0 + h0 * r1) * n + h0 * r0 ==
-     			    (h2 * r0) * (n * n) + (h0 * r1 + h1 * r0 + h2 * (5 * x)) * n + 
-    			   (h0 * r0 + h1 * (5 * x)) + ((h2*n + h1) *x)*p)) =
-       assert_by_tactic canon ((h2 * n + h1) * ((p+5) * x) == (h2 * n + h1) * 5 * x + ((h2*n + h1)*x)*p);
-
-       (*rewrite the equality *)
-       assert((h2 * n + h1) * ((p+5) * x) + ((h2 * r0) * (n * n) + (h1 * r0 + h0 * r1) * n + h0 * r0) == 
-    		  (h2 * n + h1) * 5 * x + ((h2*n + h1)*x)*p + ((h2 * r0) * (n * n) + (h1 * r0 + h0 * r1) * n + h0 * r0));
-       
-       (* this is just swapping things, doing it manually is faster. wrap c in parentheses to get a 10s boost.*)
-       swap_add ((h2 * n + h1) * 5 * x) (((h2*n + h1)*x)*p) ((h2 * r0) * (n * n) + (h1 * r0 + h0 * r1) * n + h0 * r0);
-
-       let helper_lemma_3 (y:int) : Lemma
-    	 (ensures (((h2 * n + h1) * 5 * x + y + (h1*r0 + h0*r1)*n + h0*r0  ==
-       			      (y + (h0 * r1 + h1 * r0 + h2 * (5 * x)) * n + (h0 * r0 + h1 * (5 * x)))))) =
-       assert_by_tactic canon ((h2 * n + h1) * 5 * x + y + (h1*r0 + h0*r1)*n + h0*r0  ==
-       			      (y + (h0 * r1 + h1 * r0 + h2 * (5 * x)) * n + (h0 * r0 + h1 * (5 * x))))
-       in 
-    	 helper_lemma_3 ((h2 * r0) * (n*n))
-    in
-    helper_lemma_2 (r1/4);
-   
-    (* proof that h*r = result of helper_lemma_2*)
-      assert (h*r == (h2 * r0) * (n * n) + (h0 * r1 + h1 * r0 + h2 * (5 * (r1/4))) * n + 
-      			   (h0 * r0 + h1 * (5 * (r1/4))) + ((h2*n + h1) *(r1/4))*p);
-    
-    (* unfold definition of hh *)
-      assert (hh == (h2*r0)*(n*n) + (h0*r1+h1*r0+h2*(r1+(r1/4)))*n + h0*r0 + h1*(r1+(r1/4)));
-    
-    (* proof that r1+(r1/4) = 5*(r1/4) *)
-      comm_plus #r1 #(r1/4);
-      division_addition_lemma r1 4 r1; // (r1 + r1*4)/4 = (r1/4) + r1
-      assert_norm (r1 + 4*r1 == 5*r1);
-      lemma_mul_div_sep 5 4 r1;
-      assert (r1 + (r1/4) = 5*(r1/4));
-      
-    (* proof that hh == h*r - ((h2*n+h1)*(r1/4))*p*)
-      assert (hh == (h2 * r0) * (n * n) + (h0 * r1 + h1 * r0 + h2 * (5 * (r1/4))) * n + 
-    			   h0*r0 + h1 * (5 * (r1/4)));    
-    (* proof that ((h2*n + h1)*(r1/4))*p % p = 0 *)
-
-    // not sure how to prove that, and stdlib seems to require that it's nat.
+let lemma_poly_multiply (n:int) (p:pos) (r:int) (h:int) (r0:int) (r1:nat) (h0:int) (h1:int) 
+			(h2:int) (s1:int) (d0:int) (d1:int) (d2:int) (hh:int) =
+  let helper_lemma (x:nat) (y:int) : Lemma 
+    (ensures ((h2*n + h1)*((p+5)*x) + y + (h1*r0 + h0*r1)*n + h0*r0 ==
+     	      y + (h0*r1 + h1*r0 + h2*(5*x))* n + 
+    	      (h0*r0 + h1*(5*x)) + ((h2*n + h1)*x)*p)) =
+     assert_by_tactic canon ((h2*n+h1)*((p+5)*x) == (h2*n+h1)*5*x + ((h2*n+h1)*x)*p);
+    calc (
+      (h2*n + h1)*((p+5)*x) + (y + (h1*r0 + h0*r1)*n + h0*r0)
+      &= (h2*n + h1)*5*x + ((h2*n + h1)*x)*p + (y + (h1*r0 + h0*r1)*n + h0*r0) &| using z3
+      &= (h2*n + h1)*5*x + (y + (h1*r0 + h0*r1)*n + h0*r0) + ((h2*n + h1)*x)*p &| 
+      	 using (swap_add ((h2*n + h1)*5*x) 
+			 (((h2*n + h1)*x)*p)
+      			 ((h2*r0)*(n*n) + (h1*r0 + h0*r1)*n + h0*r0))
+      &= y + (h0*r1 + h1*r0 + h2*(5*x))*n + (h0*r0 + h1*(5*x)) + ((h2*n + h1)*x)*p &|| canon
+      )
+  in
+    calc(  
+      h*r 
+      &= (h2*(n*n) + h1*n + h0)*(r1*n + r0) &| using z3
+      &= (h2*n+h1)*((n*n)*r1)+(h2*r0)*(n*n)+(h1*r0+h0*r1)*n+h0*r0 &|| canon
+      &= ((h2*n+h1)*((p+5)*(r1/4)))+(h2*r0)*(n*n)+ 
+    	 (h1*r0+h0*r1)*n + h0*r0 &| using (slash_star_axiom (n*n) 4 (p+5);
+					   lemma_mul_div_comm (p+5) 4 r1; 
+					   z3)
+      &= (h2*r0)*(n*n) + (h0*r1 + h1*r0 + h2*(5*(r1/4)))*n + 
+      	 (h0*r0 + h1*(5*(r1/4))) + ((h2*n + h1)*(r1/4))*p  &| using (helper_lemma (r1/4)
+								       ((h2*r0)*(n*n)); z3)
+     );
+      calc(
+      	r1 + (r1/4) 
+      	&= 5*(r1/4) &| using (comm_plus #r1 #(r1/4);
+      		              division_addition_lemma r1 4 r1;
+      			      lemma_mul_div_sep 5 4 r1)
+      );
+    // assumptions due to library requiring nats, can we switch to nats?
       assume ((h2*n + h1) >= 0); 
       assume ((h2*n+h1)*(r1/4) >= 0);
+      assume ((h2*r0)*(n*n) + (h0*r1 + h1*r0 + h2*(5*(r1/4)))*n + (h0*r0 + h1*(5*(r1/4))) >= 0);
+      assert (hh == (h2*r0)*(n*n) + (h0*r1 + h1*r0 + h2*(5*(r1/4)))*n + 
+    			   h0*r0 + h1*(5*(r1/4)));
+    (* proof that ((h2*n + h1)*(r1/4))*p % p = 0 *)
       multiple_modulo_lemma ((h2*n + h1)*(r1/4)) p;
-
     (* and (a+b*p)%p = a%p*)
-    
-      assume ((h2 * r0) * (n * n) + (h0 * r1 + h1 * r0 + h2 * (5 * (r1/4))) * n + (h0 * r0 + h1 * (5 * (r1/4))) >= 0);
-      lemma_mod_plus ((h2 * r0) * (n * n) + (h0 * r1 + h1 * r0 + h2 * (5 * (r1/4))) * n + (h0 * r0 + h1 * (5 * (r1/4))))
-      	((h2*n + h1) *(r1/4)) p;
+      lemma_mod_plus ((h2*r0)*(n*n) + (h0*r1 + h1*r0 + h2*(5*(r1/4)))*n + (h0*r0 + h1*(5*(r1/4))))
+      	((h2*n + h1)*(r1/4)) p;
       assert ((h*r) % p == hh % p)
 
 let lemma_poly_reduce (n:int) (p:int) (h:int) (h2:int) (h10:int) (c:int) (hh:int) =
